Strata/DL/Lambda/LExprEval.lean
@@ -68,6 +68,7 @@ def eql (F : @Factory T.base) (e1 e2 : LExpr T) : Option Bool :=
   else
   -- Disproving equality is harder, we have several special cases
   match _he: e1, e2 with
+  -- Case 1: Syntactic inequality of (non-real) constants implies semantic inequality
   | .const _ c1, .const _ c2 =>
     match c1, c2 with
     | .realConst _, .realConst _ => none
